Cleans working file #2

newio/DM1.fst
@@ -115,59 +115,38 @@ let lift_pure_dm (a : Type) (w : pure_wp a) (f:(eqtype_as_type unit -> PURE a w)
 
 ////////////////////////////////////////////////////////////////////////////////////////
 
-unfold
-let histq a (q:pure_post a) = hist (v:a{q v})
-
-unfold
-let eq_post (x y:'a) : Type0 = x == y
-
-unfold
-let histq_return (x:'a) : histq 'a (eq_post x) =
-  hist_return x
-
-let dmq (a:Type) (q:pure_post a) (wp:histq a q) = 
-  dm (v:a{q v}) wp 
-
-let dmq_return (a:Type) (x:a) : dmq a (eq_post x) (histq_return x) = 
-  dm_return _ x
-
-unfold
-let bind_post (#a #b:Type) (q1:pure_post a) (q2:a -> pure_post b)
-  : pure_post b
-  = fun y -> exists (x:a{q1 x}). q2 x y
-
-let lemma_recast_wp000
-  (a b:Type)
-  (q1:pure_post a) (q2:a -> pure_post b)
-  (xwp:(x:a{q1 x}) -> histq b (q2 x)) 
-  (x: a{q1 x})
-  (p1 p2 : hist_post (v:b{bind_post q1 q2 v}))
-  (h:trace) :
-  Lemma
-    (requires (p1 `hist_post_ord` p2 /\ xwp x (fun lt r -> p1 lt r) h))
-    (ensures (xwp x (fun lt r -> p2 lt r) h)) = ()
-
-let recast_wp
-  (a b:Type)
-  (q1:pure_post a) (q2:a -> pure_post b)
-  (wp2:(x:a) -> histq b (q2 x)) 
-  (x: a{q1 x}) :
-  Tot (hist (v:b{bind_post q1 q2 v})) = 
-  Classical.forall_intro_3 (Classical.move_requires_3 (lemma_recast_wp000 a b q1 q2 wp2 x));
-  fun p -> wp2 x (fun lt (r: b{q2 x r}) -> p lt r)
-
 let io_subcomp (a:Type)
   (q1:pure_post a) (q2:pure_post a)
   (m : io (v:a{q1 v})) :
   Pure (io (v:a{q2 v})) 
     (requires (forall x. q1 x ==> q2 x))
-    (ensures (fun _ -> True)) =
+    (ensures (fun r -> True)) =
   admit ();
   m
 
 unfold
-let hist_ordp 
-  (q1:pure_post 'a) (q2:pure_post 'a)
+let pure_post_return (x:'a) : pure_post 'a = fun y -> x == y
+
+unfold
+let pure_post_bind (#a #b:Type) (q1:pure_post a) (q2:a -> pure_post b) : pure_post b =
+  fun y -> exists (x:a{q1 x}). q2 x y
+
+unfold
+let pure_post_if_then_else (q1 q2:pure_post 'a) (b:bool) : pure_post 'a =
+  fun x -> (b ==> q1 x) /\ ((~b) ==> q2 x)
+
+/////////////////////////////////////////////////////////////////////////////////////
+
+(** Later we refine the output type of the dijkstra monad with the pure post condition (q),
+which forces us to index the dijkstra monad by a weakest-precondition of type `hist (v:a{q v})`.
+For cleanliness reasons, we define a synonym for that, called `histq`. **)
+
+unfold
+let histq a (q:pure_post a) = hist (v:a{q v})
+
+unfold
+let histq_ord
+  (#q1:pure_post 'a) (#q2:pure_post 'a)
   (wp1: histq 'a q1) 
   (wp2: histq 'a q2) :
   Pure Type0
@@ -176,59 +155,104 @@ let hist_ordp
   forall h (p:hist_post (v:'a{q1 v})). 
     wp1 p h ==> wp2 (fun lt (r:'a{q2 r}) -> p lt (r <: (x:'a{q1 x}))) h
 
-let dm_subcompp (a:Type) 
+unfold
+let histq_return (x:'a) : histq 'a (pure_post_return x) =
+  hist_return x
+
+let lemma_histq_subcomp_post
+  (a b:Type)
+  (q1:pure_post a) (q2:a -> pure_post b)
+  (wp:(x:a{q1 x}) -> histq b (q2 x)) 
+  (x: a{q1 x})
+  (p1 p2 : hist_post (v:b{pure_post_bind q1 q2 v}))
+  (h:trace) :
+  Lemma
+    (requires (p1 `hist_post_ord` p2 /\ wp x (fun lt r -> p1 lt r) h))
+    (ensures (wp x (fun lt r -> p2 lt r) h)) = ()
+
+unfold
+let histq_subcomp_bind
+  (a b:Type)
+  (q1:pure_post a) (q2:a -> pure_post b)
+  (wp2:(x:a) -> histq b (q2 x)) 
+  (x: a{q1 x}) :
+  Tot (histq b (pure_post_bind q1 q2)) = 
+  Classical.forall_intro_3 (Classical.move_requires_3 (lemma_histq_subcomp_post a b q1 q2 wp2 x));
+  fun p -> wp2 x (fun lt (r: b{q2 x r}) -> p lt r)
+
+unfold
+let histq_if_then_else (q1 q2:pure_post 'a) (wp1:histq 'a q1) (wp2:histq 'a q2) (b:bool) : histq 'a (pure_post_if_then_else q1 q2 b) by (
+  explode ();
+  dump "H"
+)=
+  admit ();
+  (** TODO: show that histq_if_then_else is monotonic **)
+  fun (p:trace -> (x:'a{pure_post_if_then_else q1 q2 b x}) -> Type0) h -> (b ==> wp1 p h) /\ ((~b) ==> wp2 p h)
+
+unfold
+let histq_for_pure (#a:Type) q : histq a q = fun p h -> forall (r:a{q r}). p [] r
+
+let dm_subcomp_histq (a:Type) 
   (q1:pure_post a) (q2:pure_post a)
   (wp1: histq a q1) 
   (wp2: histq a q2)
   (f : dm (v:a{q1 v}) wp1) :
   Pure (dm (v:a{q2 v}) wp2)
-    (requires ((forall x. q1 x ==> q2 x) /\ hist_ordp q2 q1 wp2 wp1))
+    (requires ((forall x. q1 x ==> q2 x) /\ wp2 `histq_ord` wp1))
     (ensures fun _ -> True) =
-  let m = io_subcomp a q1 q2 f in
   assert (wp1 `hist_ord` (theta f));
-  assert (wp2 `hist_ordp q2 q1` wp1);
+  assert (wp2 `histq_ord` wp1);
+
+  let m = io_subcomp a q1 q2 f in
   assert (wp2 `hist_ord` (theta m));
   m
+
+/////////////////////////////////////////////////////////////////////////////
+
+let dmq (a:Type) (q:pure_post a) (wp:histq a q) = 
+  dm (v:a{q v}) wp 
+
+let dmq_return (a:Type) (x:a) : dmq a (pure_post_return x) (histq_return x) = 
+  dm_return _ x
 
 let dmq_bind (a b:Type)
   (q1:pure_post a) (q2:a -> pure_post b)
   (wp1:histq a q1) (wp2:(x:a) -> histq b (q2 x))
   (f:dmq a q1 wp1) 
   (g:(x:a{q1 x}) -> dmq b (q2 x) (wp2 x)) :
-  Tot (dmq b (bind_post q1 q2) (hist_bind wp1 (recast_wp a b q1 q2 wp2))) =
+  Tot (dmq b (pure_post_bind q1 q2) (hist_bind wp1 (histq_subcomp_bind a b q1 q2 wp2))) =
     dm_bind 
       (v:a{q1 v})
-      (v:b{bind_post q1 q2 v})
+      (v:b{pure_post_bind q1 q2 v})
       wp1
-      (recast_wp a b q1 q2 wp2)
+      (histq_subcomp_bind a b q1 q2 wp2)
       f
       (fun (x:a{q1 x}) -> 
-        dm_subcompp b
-         (q2 x) (bind_post q1 q2)
+        dm_subcomp_histq b
+         (q2 x) (pure_post_bind q1 q2)
          (wp2 x)
-         (recast_wp a b q1 q2 wp2 x)
+         (histq_subcomp_bind a b q1 q2 wp2 x)
          (g x))
 
 let dmq_subcomp (a:Type) (q1 q2:pure_post a) (wp1:hist (v:a{q1 v})) (wp2:hist (v:a{q2 v})) (f:dmq a q1 wp1) :
   Pure (dmq a q2 wp2)
     (requires (
       (forall x. q1 x ==> q2 x) /\
-      (hist_ordp q2 q1 wp2 wp1)))
+      (wp2 `histq_ord` wp1)))
     (ensures fun _ -> True) =
-  dm_subcompp a q1 q2 wp1 wp2 f
+  dm_subcomp_histq a q1 q2 wp1 wp2 f
 
 ///////////////////////////////////////////////////////////////////////////
 
+unfold
+let pure_pre_bind (#a:Type) (p1:pure_pre) (q1:pure_post a) (p2:a -> pure_pre) : pure_pre =
+  p1 /\ (forall x. q1 x ==> p2 x)
 
 let pdmq (a:Type) (p:pure_pre) (q:pure_post a) (wp:histq a q) = 
   squash p -> dmq a q wp 
 
-let pdmq_return (a:Type) (x:a) : pdmq a True (eq_post x) (histq_return x) = 
+let pdmq_return (a:Type) (x:a) : pdmq a True (pure_post_return x) (histq_return x) = 
   fun _ -> dmq_return _ x
-
-unfold
-let bind_pre (#a:Type) (p1:pure_pre) (q1:pure_post a) (p2:a -> pure_pre) : pure_pre =
-  p1 /\ (forall x. q1 x ==> p2 x)
 
 let pdmq_bind (a b:Type)
   (p1:pure_pre) (p2:a -> pure_pre)
@@ -236,8 +260,8 @@ let pdmq_bind (a b:Type)
   (wp1:histq a q1) (wp2:(x:a) -> histq b (q2 x))
   (f:pdmq a p1 q1 wp1) 
   (g:(x:a) -> pdmq b (p2 x) (q2 x) (wp2 x)) :
-  Tot (pdmq b (bind_pre p1 q1 p2) (bind_post q1 q2) (hist_bind wp1 (recast_wp a b q1 q2 wp2))) =
-  fun (pre:squash (bind_pre p1 q1 p2)) ->
+  Tot (pdmq b (pure_pre_bind p1 q1 p2) (pure_post_bind q1 q2) (hist_bind wp1 (histq_subcomp_bind a b q1 q2 wp2))) =
+  fun (pre:squash (pure_pre_bind p1 q1 p2)) ->
   dmq_bind a b q1 q2 wp1 wp2 (f pre) (fun (x:a{q1 x}) -> g x pre)
 
 let pdmq_subcomp (a:Type) (p1 p2:pure_pre) (q1 q2:pure_post a) (wp1:hist (v:a{q1 v})) (wp2:hist (v:a{q2 v})) (f:pdmq a p1 q1 wp1) :
@@ -245,23 +269,9 @@ let pdmq_subcomp (a:Type) (p1 p2:pure_pre) (q1 q2:pure_post a) (wp1:hist (v:a{q1
     (requires (
       (p2 ==> p1) /\
       (forall x. q1 x ==> q2 x) /\
-      (hist_ordp q2 q1 wp2 wp1)))
+      (wp2 `histq_ord` wp1)))
     (ensures fun _ -> True) =
-  fun _ ->
-    dmq_subcomp a q1 q2 wp1 wp2 (f ())
-
-unfold
-let q_if_then_else (q1 q2:pure_post 'a) (b:bool) : pure_post 'a =
-  fun x -> (b ==> q1 x) /\ ((~b) ==> q2 x)
-
-unfold
-let histq_if_then_else (q1 q2:pure_post 'a) (wp1:histq 'a q1) (wp2:histq 'a q2) (b:bool) : histq 'a (q_if_then_else q1 q2 b) by (
-  explode ();
-  dump "H"
-)=
-  admit ();
-  (** TODO: show that histq_if_then_else is monotonic **)
-  fun (p:trace -> (x:'a{q_if_then_else q1 q2 b x}) -> Type0) h -> (b ==> wp1 p h) /\ ((~b) ==> wp2 p h)
+  fun _ -> dmq_subcomp a q1 q2 wp1 wp2 (f ())
   
 unfold
 let pdmq_if_then_else 
@@ -275,7 +285,7 @@ let pdmq_if_then_else
   (b : bool) : Type =
   pdmq a
     ((b ==> p1) /\ ((~b) ==> p2)) 
-    (q_if_then_else q1 q2 b)
+    (pure_post_if_then_else q1 q2 b)
     (histq_if_then_else q1 q2 wp1 wp2 b)
 
 total
@@ -301,18 +311,24 @@ effect IO
     (fun _ -> True)
     (fun (p:hist_post a) (h:trace) -> pre h /\ (forall lt r. post h lt r ==>  p lt r)) 
 
-let trivial_wp (#a:Type) q : histq a q = fun p h -> forall (r:a{q r}). p [] r
 
 unfold let as_requires (#a: Type) (wp: pure_wp a) = wp (fun x -> True)
 unfold let as_ensures (#a: Type) (wp: pure_wp a) (x: a) = ~(wp (fun y -> (y =!= x)))
 
-let lift_pure_pdmq (a : Type) (w : pure_wp a) (f:(eqtype_as_type unit -> PURE a w)) : 
-  pdmq a (as_requires w) (as_ensures w) (trivial_wp (as_ensures w)) =
-  fun _ ->
+(** histq_for_pure is labeled with unfold, but when trying to prove the lift, it confuses
+the SMT. Therefore, this is just a trick to get an automated proof of the lift **)
+let histq_for_pure0 = histq_for_pure
+let lift_pure_pdmq0 (a : Type) (w : pure_wp a) (f:(eqtype_as_type unit -> PURE a w)) : 
+  pdmq a (as_requires w) (as_ensures w) (histq_for_pure0 (as_ensures w)) =
+  fun (pre:squash (as_requires w)) ->
     FStar.Monotonic.Pure.elim_pure_wp_monotonicity_forall ();
     let r = f () in
-    let r' = dmq_return a r in
+    let r' = dmq_return _ r in
     dmq_subcomp _ _ _ _ _ r'
+
+let lift_pure_pdmq (a : Type) (w : pure_wp a) (f:(eqtype_as_type unit -> PURE a w)) : 
+  pdmq a (as_requires w) (as_ensures w) (histq_for_pure (as_ensures w)) =
+    lift_pure_pdmq0 a w f
 
 sub_effect PURE ~> IOwp = lift_pure_pdmq
 
@@ -330,7 +346,7 @@ let test' () : IO unit (fun _ -> True) (fun _ _ _ -> True) =
   pure_lemma ();
   some_f ()
 
-let test'' () : IO unit (fun _ -> True) (fun _ _ _ -> True) by (explode ())=
+let test'' () : IO unit (fun _ -> True) (fun _ _ _ -> True) =
   pure_lemma ();
   some_f ();
   assert p';
@@ -340,17 +356,16 @@ let static_cmd
   (cmd : io_cmds)
   (argz : io_args cmd) :
   IO (io_resm cmd)
-    (requires (fun h -> io_pres cmd argz h))
+    (requires (fun h -> io_pre cmd argz h))
     (ensures (fun h lt r ->
         lt == [convert_call_to_event cmd argz r])) =
   IOwp?.reflect (fun _ -> io_call cmd argz)
 
-let testStatic3 (fd:file_descr) : IO unit (fun h -> is_open fd h) (fun h lt r -> ~(is_open fd (trace_append h lt))) by (explode ()) =
+let testStatic3 (fd:file_descr) : IO unit (fun h -> is_open fd h) (fun h lt r -> ~(is_open fd (trace_append h lt))) =
   let _ = static_cmd Close fd in
   ()
 
-let testStatic2 () : IO unit (fun _ -> True) (fun _ _ _ -> True) by (
-  explode ()) =
+let testStatic2 () : IO unit (fun _ -> True) (fun _ _ _ -> True) =
   let fd = static_cmd Openfile "../Makefile" in
   if Some? fd then begin (** test if Openfile was successful **)
     let msg = static_cmd Read (Some?.v fd) in
